Moved to non-extended operations + Extraction + Bounds-checking

src/Assembly/Pipeline.v
@@ -1,159 +1,86 @@
-Require Import Coq.ZArith.BinInt.
+Require Export Crypto.Assembly.QhasmCommon.
+Require Export Crypto.Assembly.PhoasCommon.
+Require Export Crypto.Assembly.HL.
+Require Export Crypto.Assembly.LL.
+Require Export Crypto.Assembly.Compile.
+Require Export Crypto.Assembly.Conversions.
+Require Export Crypto.Assembly.StringConversion.
+Require Export Crypto.Assembly.State.
 
-Require Import Crypto.Assembly.QhasmCommon.
-Require Import Crypto.Assembly.PhoasCommon.
-Require Import Crypto.Assembly.HL.
-Require Import Crypto.Assembly.LL.
-Require Import Crypto.Assembly.Compile.
-Require Import Crypto.Assembly.Conversions.
-Require Import Crypto.Assembly.StringConversion.
-Require Import Crypto.Assembly.State.
+Require Export Crypto.Util.Notations.
+Require Export Crypto.Util.LetIn.
 
-Require Import Crypto.Util.Notations.
-Require Import Crypto.Util.LetIn.
+Require Export Coq.ZArith.BinInt.
 
-Module SimpleExample.
-  Definition bits: nat := 32.
-  Definition width: Width bits := W32.
+Require Export ExtrOcamlBasic.
+Require Export ExtrOcamlString.
 
-  Definition hlProg: NAry 1 Z (@HL.expr Z (@LL.arg Z Z) TT) :=
-    fun x => HL.Binop OPadd (HL.Const x) (HL.Const 5%Z).
+Module Type Expression.
+  Parameter bits: nat.
+  Parameter width: Width bits.
+  Parameter inputs: nat.
+  Parameter ResultType: type.
+  Parameter hlProg: NAry inputs Z (@HL.expr Z (@LL.arg Z Z) ResultType).
+  Parameter inputUpperBounds: list (@WordRangeOpt bits).
+End Expression.
 
-  Definition llProg: NAry 1 Z (@LL.expr Z Z TT) :=
+Module Pipeline (Input: Expression).
+  Export Input.
+
+  Definition llProg: NAry inputs Z (@LL.expr Z Z ResultType) :=
     liftN CompileHL.compile hlProg.
 
-  Definition wordProg: NAry 1 (@CompileLL.WArg bits TT) (@LL.expr _ _ TT) :=
+  Definition wordProg: NAry inputs (@CompileLL.WArg bits TT) (@LL.expr _ _ ResultType) :=
     NArgMap (fun x => Z.of_N (wordToN (LL.interp_arg (t := TT) x))) (
       liftN (LLConversions.convertZToWord bits) llProg).
 
   Definition qhasmProg := CompileLL.compile (w := width) wordProg.
 
-  Definition qhasmString: option string :=
-    Eval cbv in match qhasmProg with
-                | Some (p, _) => StringConversion.convertProgram p
-                | None => None
-                end.
-
-  Section BoundsCheck.
-    Definition R := @WordRangeOpt bits.
-
-    Definition rangeProg: NAry 1 R (@LL.expr R R TT) :=
-      NArgMap (fun x => getOrElse (Z.of_N (N.pred (Npow2 bits)))
-                               (option_map Z.of_N (getUpperBoundOpt x))) (
-                liftN (LLConversions.convertZToWordRangeOpt bits) llProg).
-
-    Definition rangeValid: NAry 1 R Prop :=
-      liftN (LLConversions.check) rangeProg.
-
-    (* Check that our bounds are valid for any Z in 0..2^31 *)
-    Lemma rangeValidAny: rangeValid (makeRange 0 (Z.shiftl 1 31))%Z.
-    Proof. cbv; intuition. Qed.
-  End BoundsCheck.
-End SimpleExample.
-
-Module GF25519.
-  Require Import Crypto.Spec.ModularArithmetic.
-  Require Import Crypto.CompleteEdwardsCurve.ExtendedCoordinates.
-  Require Import Crypto.ModularArithmetic.ModularBaseSystem.
-  Require Import Crypto.Specific.GF25519.
-
-  (* Computing the length first is necessary to make this run in tolerable time on 8.6 *)
-  Definition q : Z := (2 ^ 255 - 19)%Z.
-  Definition d : F q := (F.opp (F.of_Z q 121665%Z) / (F.of_Z q 121666%Z))%F.
-
-  Definition twice_d' := Eval cbv [length params25519 ModularBaseSystemOpt.limb_widths_from_len ModularBaseSystem.encode ModularBaseSystemList.encode PseudoMersenneBaseParams.limb_widths] in ModularBaseSystem.encode(modulus:=q) (d + d)%F.
-  Definition twice_d : fe25519 := Eval vm_compute in twice_d'.
-
-  Definition ge25519_add' :=
-    Eval cbv beta delta [Extended.add_coordinates fe25519 add mul sub Let_In twice_d] in
-      @Extended.add_coordinates fe25519 add sub mul twice_d.
-
-  Definition ResultType: type.
-  Proof.
-    let T' := type of (twice_d, twice_d, twice_d, twice_d) in
-    let T := eval vm_compute in T' in
-    let t := HL.reify_type T in
-    exact t.
-  Defined.
-
-  Definition ge25519_ast' (P Q: @interp_type Z ResultType) :
-      { r: @HL.expr Z (@interp_type Z) ResultType
-      | HL.interp (E := ZEvaluable) (t := ResultType) r
-        = ge25519_add' P Q }.
-  Proof.
-    vm_compute in P, Q; repeat
-      match goal with
-      | [x:?T |- _] =>
-        lazymatch T with
-        | Z => fail
-        | prod _ _ => destruct x
-        | _ => clear x
-        end
-      end.
-
-    eexists.
-    cbv beta delta [ge25519_add'].
-
-    let R := HL.rhs_of_goal in
-    let X := HL.reify (@interp_type Z) R in idtac;
-    transitivity (HL.interp (E := ZEvaluable) (t := ResultType) X);
-      [reflexivity|].
-
-    cbv iota beta delta [
-          interp_type interp_binop HL.interp
-          Z.land ZEvaluable eadd esub emul eshiftr eand].
-    reflexivity.
-  Defined.
-
-  Definition ge25519_ast (P Q: @interp_type Z ResultType) :=
-    proj1_sig (ge25519_ast' P Q).
-
-  Definition bits: nat := 64.
-  Definition width: Width bits := W64.
-
-  Definition lift10 {T} (F: (Z*Z*Z*Z*Z*Z*Z*Z*Z*Z) -> T) := fun (a b c d e f g h i j: Z) =>
-      F (a, b, c, d, e, f, g, h, i, j).
-
-  Definition hlProg': NAry 80 Z (@HL.expr Z (@interp_type Z) ResultType) :=
-    lift10 (fun px => lift10 (fun py => lift10 (fun pz => lift10 (fun pt =>
-    lift10 (fun qx => lift10 (fun qy => lift10 (fun qz => lift10 (fun qt =>
-    ge25519_ast (px, py, pz, pt) (qx, qy, qz, qt))))))))).
-
-  Definition hlProg: NAry 80 Z (@HL.expr Z (@LL.arg Z Z) ResultType).
-    refine (liftN (HLConversions.mapVar _ _) hlProg'); intro t;
-      [ refine LL.uninterp_arg | refine LL.interp_arg ].
-  Defined.
-
-  Definition llProg: NAry 80 Z (@LL.expr Z Z ResultType) :=
-    Eval vm_compute in (liftN CompileHL.compile hlProg).
-
-  (* Don't vm_compute because it'll stack overflow (!!) *)
-  Definition wordProg: NAry 80 (@CompileLL.WArg bits TT) (@LL.expr _ _ ResultType) :=
-    NArgMap (fun x => Z.of_N (wordToN (LL.interp_arg (t := TT) x))) (
-      liftN (LLConversions.convertZToWord bits) llProg).
-
-  Definition qhasmProg :=
-    Eval vm_compute in (CompileLL.compile (w := width) wordProg).
-
-  Definition qhasmString: option string :=
+  Definition qhasmString : option string :=
     match qhasmProg with
     | Some (p, _) => StringConversion.convertProgram p
     | None => None
     end.
 
-  Section BoundsCheck.
-    Definition R := @WordRangeOpt bits.
+  Definition Range := @WordRangeOpt bits.
 
-    Definition rangeProg: NAry 80 R (@LL.expr R R ResultType) :=
-      NArgMap (fun x => getOrElse (Z.of_N (N.pred (Npow2 bits)))
-          (option_map Z.of_N (getUpperBoundOpt x))) (
-        liftN (LLConversions.convertZToWordRangeOpt bits) llProg).
+  Definition rangeProg: NAry inputs Range (@LL.expr Range Range ResultType) :=
+    NArgMap (fun x =>
+        getOrElse (Z.of_N (N.pred (Npow2 bits)))
+                  (option_map Z.of_N (getUpperBoundOpt x))) (
+      liftN (LLConversions.convertZToWordRangeOpt bits) llProg).
 
-    Definition rangeValid: NAry 80 R Prop :=
-        liftN (LLConversions.check) rangeProg.
+  Definition rangeCheck: NAry inputs Range bool :=
+    liftN (LLConversions.check') rangeProg.
 
-    (* TODO: what are our prior ranges on the inputs?
-    Lemma rangeValidAny: rangeValid (makeRange 0 (Z.shiftl 1 31))%Z.
-    Proof. cbv; intuition. Qed. *)
-  End BoundsCheck.
-End GF25519.
+  Definition rangeValid: bool :=
+    let F := (fix rangeValid' k ins (f: NAry k Range bool) :=
+        (match k as k' return NAry k' Range bool -> bool with
+        | O => id
+        | S m => fun f' =>
+          match ins with
+          | cons x xs => rangeValid' m xs (f' x)
+          | nil => rangeValid' m nil (f' anyWord)
+          end
+        end f)) in
+
+    F _ inputUpperBounds rangeCheck.
+End Pipeline.
+
+Module SimpleExample.
+  Module SimpleExpression <: Expression.
+    Definition bits: nat := 32.
+    Definition width: Width bits := W32.
+    Definition inputs: nat := 1.
+    Definition ResultType := TT.
+
+    Definition hlProg: NAry 1 Z (@HL.expr Z (@LL.arg Z Z) TT) :=
+        Eval vm_compute in (fun x => HL.Binop OPadd (HL.Const x) (HL.Const 5%Z)).
+
+    Definition inputUpperBounds: list (@WordRangeOpt bits) := nil.
+  End SimpleExpression.
+
+  Module SimplePipeline := Pipeline SimpleExpression.
+
+  Export SimplePipeline.
+End SimpleExample.
