src/Assembly/GF25519.v
@@ -1,0 +1,256 @@
+Require Import Crypto.Assembly.Pipeline.
+
+Require Import Crypto.Spec.ModularArithmetic.
+Require Import Crypto.ModularArithmetic.ModularBaseSystem.
+Require Import Crypto.Specific.GF25519.
+Require Import Crypto.Util.Tuple.
+
+Module GF25519.
+  Definition q : Z := (2 ^ 255 - 19)%Z.
+  Definition d : F q := (F.opp (F.of_Z q 121665%Z) / (F.of_Z q 121666%Z))%F.
+
+  Definition twice_d' := Eval cbv [length params25519 ModularBaseSystemOpt.limb_widths_from_len ModularBaseSystem.encode ModularBaseSystemList.encode PseudoMersenneBaseParams.limb_widths] in ModularBaseSystem.encode(modulus:=q) (d + d)%F.
+  Definition twice_d : fe25519 := Eval vm_compute in twice_d'.
+
+  Definition FE: type.
+  Proof.
+    let T := eval vm_compute in fe25519 in
+    let t := HL.reify_type T in
+    exact t.
+  Defined.
+
+  Definition liftFE {T} (F: @interp_type Z FE -> T) :=
+    fun (a b c d e f g h i j: Z) => F (a, b, c, d, e, f, g, h, i, j).
+
+  Fixpoint makeBoundList {n} k (b: @WordRangeOpt n) :=
+    match k with
+    | O => nil
+    | S k' => cons b (makeBoundList k' b)
+    end.
+
+  Module AddExpr <: Expression.
+    Definition bits: nat := 64.
+    Definition inputs: nat := 20.
+    Definition width: Width bits := W64.
+    Definition ResultType := FE.
+    Definition inputUpperBounds: list (@WordRangeOpt bits) :=
+      makeBoundList 20 (makeRange 0 (Z.of_N (Npow2 28))).
+
+    Definition ge25519_add_expr :=
+        Eval cbv beta delta [fe25519 add mul sub Let_In twice_d] in add.
+
+    Definition ge25519_add' (P Q: @interp_type Z FE) :
+        { r: @HL.expr Z (@interp_type Z) FE
+        | HL.interp (E := ZEvaluable) (t := FE) r = ge25519_add_expr P Q }.
+    Proof.
+        vm_compute in P, Q; repeat
+        match goal with
+        | [x:?T |- _] =>
+            lazymatch T with
+            | Z => fail
+            | prod _ _ => destruct x
+            | _ => clear x
+            end
+        end.
+
+        eexists.
+        cbv beta delta [ge25519_add_expr].
+
+        let R := HL.rhs_of_goal in
+        let X := HL.reify (@interp_type Z) R in
+        transitivity (HL.interp (E := ZEvaluable) (t := ResultType) X);
+        [reflexivity|].
+
+        cbv iota beta delta [
+            interp_type interp_binop HL.interp
+            Z.land ZEvaluable eadd esub emul eshiftr eand].
+        reflexivity.
+    Defined.
+
+    Definition ge25519_add (P Q: @interp_type Z ResultType) :=
+        proj1_sig (ge25519_add' P Q).
+
+    Definition hlProg'': NAry 20 Z (@HL.expr Z (@interp_type Z) ResultType) :=
+        liftFE (fun p => (liftFE (fun q => ge25519_add p q))).
+
+    Definition hlProg': NAry 20 Z (@HL.expr Z (@LL.arg Z Z) ResultType).
+        refine (liftN (HLConversions.mapVar _ _) hlProg''); intro t;
+        [ refine LL.uninterp_arg | refine LL.interp_arg ].
+    Defined.
+
+    Definition hlProg: NAry 20 Z (@HL.expr Z (@LL.arg Z Z) ResultType) :=
+      Eval vm_compute in hlProg'.
+  End AddExpr.
+
+  Module SubExpr <: Expression.
+    Definition bits: nat := 64.
+    Definition inputs: nat := 20.
+    Definition width: Width bits := W64.
+    Definition ResultType := FE.
+    Definition inputUpperBounds: list (@WordRangeOpt bits) :=
+      makeBoundList 20 (makeRange 0 (Z.of_N (Npow2 28))).
+
+    Definition ge25519_sub_expr :=
+        Eval cbv beta delta [fe25519 add mul sub Let_In twice_d] in sub.
+
+    Definition ge25519_sub' (P Q: @interp_type Z FE) :
+        { r: @HL.expr Z (@interp_type Z) FE
+        | HL.interp (E := ZEvaluable) (t := FE) r = ge25519_sub_expr P Q }.
+    Proof.
+        vm_compute in P, Q; repeat
+        match goal with
+        | [x:?T |- _] =>
+            lazymatch T with
+            | Z => fail
+            | prod _ _ => destruct x
+            | _ => clear x
+            end
+        end.
+
+        eexists.
+        cbv beta delta [ge25519_sub_expr].
+
+        let R := HL.rhs_of_goal in
+        let X := HL.reify (@interp_type Z) R in
+        transitivity (HL.interp (E := ZEvaluable) (t := ResultType) X);
+        [reflexivity|].
+
+        cbv iota beta delta [
+            interp_type interp_binop HL.interp
+            Z.land ZEvaluable eadd esub emul eshiftr eand].
+        reflexivity.
+    Defined.
+
+    Definition ge25519_sub (P Q: @interp_type Z ResultType) :=
+        proj1_sig (ge25519_sub' P Q).
+
+    Definition hlProg'': NAry 20 Z (@HL.expr Z (@interp_type Z) ResultType) :=
+        liftFE (fun p => (liftFE (fun q => ge25519_sub p q))).
+
+    Definition hlProg': NAry 20 Z (@HL.expr Z (@LL.arg Z Z) ResultType).
+        refine (liftN (HLConversions.mapVar _ _) hlProg''); intro t;
+        [ refine LL.uninterp_arg | refine LL.interp_arg ].
+    Defined.
+
+    Definition hlProg: NAry 20 Z (@HL.expr Z (@LL.arg Z Z) ResultType) :=
+      Eval vm_compute in hlProg'.
+  End SubExpr.
+
+  Module MulExpr <: Expression.
+    Definition bits: nat := 64.
+    Definition inputs: nat := 20.
+    Definition width: Width bits := W64.
+    Definition ResultType := FE.
+    Definition inputUpperBounds: list (@WordRangeOpt bits) :=
+      makeBoundList 20 (makeRange 0 (Z.of_N (Npow2 28))).
+
+    Definition ge25519_mul_expr :=
+        Eval cbv beta delta [fe25519 add mul sub Let_In twice_d] in mul.
+
+    Definition ge25519_mul' (P Q: @interp_type Z FE) :
+        { r: @HL.expr Z (@interp_type Z) FE
+        | HL.interp (E := ZEvaluable) (t := FE) r = ge25519_mul_expr P Q }.
+    Proof.
+        vm_compute in P, Q; repeat
+        match goal with
+        | [x:?T |- _] =>
+            lazymatch T with
+            | Z => fail
+            | prod _ _ => destruct x
+            | _ => clear x
+            end
+        end.
+
+        eexists.
+        cbv beta delta [ge25519_mul_expr].
+
+        let R := HL.rhs_of_goal in
+        let X := HL.reify (@interp_type Z) R in
+        transitivity (HL.interp (E := ZEvaluable) (t := ResultType) X);
+        [reflexivity|].
+
+        cbv iota beta delta [
+            interp_type interp_binop HL.interp
+            Z.land ZEvaluable eadd esub emul eshiftr eand].
+        reflexivity.
+    Defined.
+
+    Definition ge25519_mul (P Q: @interp_type Z ResultType) :=
+        proj1_sig (ge25519_mul' P Q).
+
+    Definition hlProg'': NAry 20 Z (@HL.expr Z (@interp_type Z) ResultType) :=
+        liftFE (fun p => (liftFE (fun q => ge25519_mul p q))).
+
+    Definition hlProg': NAry 20 Z (@HL.expr Z (@LL.arg Z Z) ResultType).
+        refine (liftN (HLConversions.mapVar _ _) hlProg''); intro t;
+        [ refine LL.uninterp_arg | refine LL.interp_arg ].
+    Defined.
+
+    Definition hlProg: NAry 20 Z (@HL.expr Z (@LL.arg Z Z) ResultType) :=
+      Eval vm_compute in hlProg'.
+  End MulExpr.
+
+  Module OppExpr <: Expression.
+    Definition bits: nat := 64.
+    Definition inputs: nat := 10.
+    Definition width: Width bits := W64.
+    Definition ResultType := FE.
+    Definition inputUpperBounds: list (@WordRangeOpt bits) :=
+      makeBoundList 10 (makeRange 0 (Z.of_N (Npow2 28))).
+
+    Definition ge25519_opp_expr :=
+        Eval cbv beta delta [fe25519 add mul sub opp Let_In twice_d] in opp.
+
+    Definition ge25519_opp' (P: @interp_type Z FE) :
+        { r: @HL.expr Z (@interp_type Z) FE
+        | HL.interp (E := ZEvaluable) (t := FE) r = ge25519_opp_expr P }.
+    Proof.
+        vm_compute in P; repeat
+        match goal with
+        | [x:?T |- _] =>
+            lazymatch T with
+            | Z => fail
+            | prod _ _ => destruct x
+            | _ => clear x
+            end
+        end.
+
+        eexists.
+        cbv beta delta [ge25519_opp_expr zero_].
+
+        let R := HL.rhs_of_goal in
+        let X := HL.reify (@interp_type Z) R in
+        transitivity (HL.interp (E := ZEvaluable) (t := ResultType) X);
+        [reflexivity|].
+
+        cbv iota beta delta [
+            interp_type interp_binop HL.interp
+            Z.land ZEvaluable eadd esub emul eshiftr eand].
+        reflexivity.
+    Defined.
+
+    Definition ge25519_opp (P: @interp_type Z ResultType) :=
+        proj1_sig (ge25519_opp' P).
+
+    Definition hlProg'': NAry 10 Z (@HL.expr Z (@interp_type Z) ResultType) :=
+        liftFE (fun p => ge25519_opp p).
+
+    Definition hlProg': NAry 10 Z (@HL.expr Z (@LL.arg Z Z) ResultType).
+        refine (liftN (HLConversions.mapVar _ _) hlProg''); intro t;
+        [ refine LL.uninterp_arg | refine LL.interp_arg ].
+    Defined.
+
+    Definition hlProg: NAry 10 Z (@HL.expr Z (@LL.arg Z Z) ResultType) :=
+      Eval vm_compute in hlProg'.
+  End OppExpr.
+
+  Module Add := Pipeline AddExpr.
+  Module Sub := Pipeline SubExpr.
+  Module Mul := Pipeline MulExpr.
+  Module Opp := Pipeline OppExpr.
+End GF25519.
+
+Extraction "GF25519Add" GF25519.Add.
+Extraction "GF25519Sub" GF25519.Sub.
+Extraction "GF25519Mul" GF25519.Mul.
+Extraction "GF25519Opp" GF25519.Opp.
